tests/lean/run/autoattach.lean
@@ -6,7 +6,7 @@ structure Tree (α : Type u) where
 def Tree.isLeaf (t : Tree α) := t.cs.isEmpty
 
 /--
-error: tactic 'fail' failed
+error: unsolved goals
 α : Type u_1
 t x✝ : Tree α
 ⊢ sizeOf x✝ < sizeOf t
@@ -15,10 +15,10 @@ t x✝ : Tree α
 def Tree.map (f : α → β) (t : Tree α) : Tree β :=
     ⟨f t.val, t.cs.map (·.map f)⟩
 termination_by t
-decreasing_by fail
+decreasing_by skip
 
 /--
-error: tactic 'fail' failed
+error: unsolved goals
 α : Type u_1
 t x✝ : Tree α
 ⊢ sizeOf x✝ < sizeOf t
@@ -27,14 +27,14 @@ t x✝ : Tree α
 def Tree.pruneRevAndMap (f : α → β) (t : Tree α) : Tree β :=
     ⟨f t.val, (t.cs.filter (not ·.isLeaf)).reverse.map (·.pruneRevAndMap f)⟩
 termination_by t
-decreasing_by fail
+decreasing_by skip
 
 structure MTree (α : Type u) where
   val : α
   cs : Array (List (MTree α))
 
 /--
-error: tactic 'fail' failed
+error: unsolved goals
 α : Type u_1
 t x✝ : MTree α
 ⊢ sizeOf x✝ < sizeOf t
@@ -43,7 +43,7 @@ t x✝ : MTree α
 def MTree.map (f : α → β) (t : MTree α) : MTree β :=
     ⟨f t.val, t.cs.map (·.map (·.map f))⟩
 termination_by t
-decreasing_by fail
+decreasing_by skip
 
 
 namespace Ex1
@@ -52,7 +52,7 @@ inductive Expression where
 | object: List (String × Expression) → Expression
 
 /--
-error: tactic 'fail' failed
+error: unsolved goals
 L : List (String × Expression)
 x : String × Expression
 ⊢ sizeOf x.snd < sizeOf (Expression.object L)
@@ -63,6 +63,6 @@ def t (exp: Expression): List String :=
   | Expression.var s => [s]
   | Expression.object L => List.foldl (fun L1 L2 => L1 ++ L2) [] (L.map (fun x => t x.2))
 termination_by exp
-decreasing_by fail
+decreasing_by skip
 
 end Ex1
